\chapter{7}{Matriser}

\begin{task}{7.4 a)}
	\[AB=\begin{mat}
		1 & 1 & 0 \\
		-2& 0 & 1 
	\end{mat}\begin{mat}
		2 & 1 \\
		0 &-1 \\
		1 & 0
	\end{mat}=
	\begin{mat}
		1\*2 & 1-1 \\
		-2\*2+1 &-2 
	\end{mat}=
	\begin{mat}
		2 & 0 \\
		-3 &-2 
	\end{mat}
	\]
	\[BA=\begin{mat}
		2 & 1 \\
		0 &-1 \\
		1 & 0
	\end{mat}\begin{mat}
		1 & 1 & 0 \\
		-2& 0 & 1
	\end{mat}=
	\begin{mat}
		2\*1-1\*2 & 2\*1 & 1 \\
		2 & 0 & -1 \\
		1 & 1 & 0
	\end{mat}=
	\begin{mat}
		0 & 2 & 1 \\
		2 & 0 &-1 \\
		1 & 1 & 0 
	\end{mat}
	\]
\end{task}

\begin{task}{b)}
	\[B^T=
	\begin{mat}
		2 & 0 & 1 \\
		1 &-1 & 0 
	\end{mat}\]
	\[A^T=
	\begin{mat}
		1 &-2 \\
		1 & 0 \\
		0 & 1
	\end{mat}\]
	\[B^TA^T=
	\begin{mat}
		2 & 0 & 1 \\
		1 &-1 & 0 
	\end{mat}
	\begin{mat}
		1 &-2 \\
		1 & 0 \\
		0 & 1
	\end{mat}=
	\begin{mat}
		2 &-2\*2+1 \\
		1-1 &-2
	\end{mat}=
	\begin{mat}
		2 &-3 \\
		0 &-2
	\end{mat}\]
	\[(AB)^T=B^TA^T\]
\end{task}

\begin{task}{7.9 a)}
	\[A=\begin{mat}
		1 & 2 & 0 \\
		4 & 1 &-1 \\
		2 & 3 & 0
	\end{mat}\]
	\[\begin{array}{lll}
		D_{11}=\begin{mat}
			1 &-1 \\
			3 & 0
		\end{mat}=3, 
		&D_{12}=\begin{mat}
			4 &-1 \\
			2 & 0
		\end{mat}=2,
		&D_{13}=\begin{mat}
			4 & 1 \\
			2 & 3
		\end{mat}=10, \\
		D_{21}=\begin{mat}
			2 & 0 \\
			3 & 0
		\end{mat}=0, 
		&D_{22}=\begin{mat}
			1 & 0 \\
			2 & 
		\end{mat}=0,
		&D_{23}=\begin{mat}
			1 & 2 \\
			2 & 3
		\end{mat}=-1, \\
		D_{31}=\begin{mat}
			2 & 0 \\
			1 &-1
		\end{mat}=-2, 
		&D_{32}=\begin{mat}
			1 & 0 \\
			4 &-1
		\end{mat}=-1,
		&D_{33}=\begin{mat}
			1 & 2 \\
			4 & 1
		\end{mat}=-7
	\end{array}\]
	\[\adj A =\begin{mat}
		3 & 0 &-2 \\
		-2& 0 & 1 \\
		10& 1 &-7
	\end{mat}\]
	\[A^{-1}=\frac{1}{\det A}\adj A= 
	\frac{1}{1\*3-2\*2}
	\begin{mat}
		3 & 0 &-2 \\
		-2& 0 & 1 \\
		10& 1 &-7
	\end{mat}=
	\begin{mat}
		-3& 0 & 2 \\
		2 & 0 &-1 \\
		-10&-1 & 7
	\end{mat}\]
\end{task}

\begin{task}{7.10}
	\[(AX+B)^{-1}=A \Leftrightarrow
	AX+B=A^{-1} \Leftrightarrow
	AX=A^{-1}-B\]
	\[A^{-1}=
	\begin{mat}
		1 & 0 &-1 \\
		1 &-1 & 0 \\
		-1& 1 & 1
	\end{mat}\]
	AnsÃ¤tt lÃ¶sning:
	\begin{align*}
		&\begin{mat}
			1 & 1 & 1 \\
			1 & 0 & 1 \\
			0 & 1 & 1
		\end{mat}
		\begin{mat}
			a & b & c \\
			d & e & f \\
			g & h & i
		\end{mat}=
		\begin{mat}
			1 & 0 &-1 \\
			1 &-1 & 0 \\
			-1& 1 & 1
		\end{mat}-
		\begin{mat}
			1 & 2 & 3 \\
			4 & 5 & 6 \\
			7 & 8 & 9
		\end{mat} \lra \\ \lra
		&\begin{mat}
			a+d+g & b+e+h & c+f+i \\
			a+g & b+h & c+i \\
			d+g & e+h & f+i
		\end{mat}=
		\begin{mat}
			0 &-2 &-4 \\
			-3&-6 &-6 \\
			-8&-7 &-8
		\end{mat} \lra \\ \lra
		&\begin{cases}
			a+d+g = 0 \\
			b+e+h = -2 \\
			c+f+i = -4 \\
			a+g = -3 \\
			b+h = -6 \\
			c+i = -6 \\
			d+g = -8 \\
			e+h = -7 \\
			f+i = -8
		\end{cases} \lra
		\begin{cases}
			a= 8\\
			b= 5\\
			c= 4\\
			d= 3\\
			e= 4\\
			f= 2\\
			g= -11\\
			h= -11\\
			i= -10
		\end{cases}
	\end{align*}
	\[X=
	\begin{mat}
	8 & 5 & 4 \\
	3 & 4 & 2 \\
	-11&-11&-10
	\end{mat}\]
\end{task}